verified/subdir.mk
@@ -63,7 +63,7 @@ $(dir)/kom_common.s.verified: $(dir)/ARMdef.verified
 $(dir)/pagedb.s.verified: $(dir)/kom_common.s.verified $(dir)/Maybe.verified $(dir)/Sets.verified
 $(dir)/kom_common.i.verified: $(dir)/ARMspartan.verified $(dir)/kom_common.s.verified $(dir)/pagedb.s.verified
 $(dir)/smcapi.s.verified: $(dir)/kom_common.s.verified $(dir)/pagedb.s.verified $(dir)/entry.s.verified
-$(dir)/smcapi.i.verified: $(dir)/smcapi.s.verified
+$(dir)/smcapi.i.verified: $(dir)/smcapi.s.verified $(dir)/entry.i.verified
 $(dir)/pagedb.i.verified: $(dir)/pagedb.s.verified $(dir)/kom_common.i.verified
 $(dir)/ptables.i.verified: $(dir)/pagedb.i.verified $(dir)/entry.s.verified $(dir)/ptebits.i.verified
 $(dir)/ptebits.i.verified: $(dir)/smcapi.s.verified $(dir)/pagedb.i.verified $(dir)/bitvectors.i.verified
